

Problem 1.

- (a) We assume the marble is a quantum particle with the given mass and energy in a well of the given length. From the energy levels of the infinite square well:

$$\begin{aligned}
 E_n &= \frac{\hbar^2 n^2 \pi^2}{2mL^2} \\
 \Rightarrow n &= \sqrt{\frac{2mL^2 E_n}{\hbar^2 \pi^2}} \\
 &= \frac{\sqrt{2mLE_n}}{\hbar \pi} \\
 &= \frac{\sqrt{2(1 \times 10^{-3} \text{kg})(1 \times 10^{-2} \text{m})(1 \times 10^{-3} \text{J})}}{(1.05 \times 10^{-34} \text{J} \cdot \text{s})\pi} \\
 &= 1.356 \times 10^{27}.
 \end{aligned}$$

- (b) The excitation energy is

$$\begin{aligned}
 E_{n+1} - E_n &= \frac{\hbar^2 \pi^2}{2mL^2} [(n+1)^2 - n^2] \\
 &= \frac{(2n+1)\hbar^2 \pi^2}{2mL^2} \\
 &= \frac{[2(1.356 \times 10^{27}) + 1](1.05 \times 10^{-34} \text{J} \cdot \text{s})^2 \pi^2}{2(1 \times 10^{-3} \text{kg})(1 \times 10^{-2} \text{m})^2} \\
 &= 0.141 \text{J}.
 \end{aligned}$$

Problem 2.

- (a) We solve the Schrödinger equation in each of the three regions. Factoring $\Psi(x, t) = \psi(x)T(t)$, we always have that $T = \exp(-iE_n t/\hbar)$. For the region in which $V = V_0$:

$$\begin{aligned}
 -\frac{\hbar^2}{2m}\psi''(x) + V_0\psi(x) &= E_n\psi(x) \\
 \Rightarrow \psi'' &= \frac{2m(V_0 - E_n)}{\hbar^2}\psi.
 \end{aligned}$$

In the middle region, the coefficient of ψ is some positive value β^2 . In the other two regions, the resulting equation for ψ is the same except $V_0 = 0$, yielding a negative coefficient k^2 . We thus have that ψ is the piecewise function

$$\psi(x) = \begin{cases} \psi^1, & x \in (-\infty, -a] \\ \psi^2, & x \in [-a, a] \\ \psi^3, & x \in [a, \infty), \end{cases}$$

where

$$\begin{aligned}
 \psi^1(x) &= Ae^{ikx} + Be^{-ikx} \\
 \psi^2(x) &= Ce^{\beta x} + De^{-\beta x} \\
 \psi^3(x) &= Ee^{ikx} + Fe^{-ikx}.
 \end{aligned}$$

The coefficient E is not to be confused with the energy E_n . Since wavefunctions are invariant under scaling, we can set $A = 1$. And as there is no possible reflection in the region $[a, \infty)$, it must be that $F = 0$. Thus we have

$$\psi^1(x) = e^{ikx} + Be^{-ikx}$$

$$\begin{aligned}\psi^2(x) &= Ce^{\beta x} + De^{-\beta x} \\ \psi^3(x) &= Ee^{ikx}.\end{aligned}$$

(b) Let $z = e^{ika}$, $w = e^{\beta a}$, $\bar{z} = 1/z$, and $\bar{w} = 1/w$. To ensure $C^0(\mathbb{R})$ continuity, we must have

$$\begin{aligned}\psi^1(-a) = \psi^2(-a) &\implies \bar{z} + Bz = C\bar{w} + Dw \\ \psi^1(a) = \psi^2(a) &\implies Cw + D\bar{w} = Ez\end{aligned}$$

(c) To ensure $C^1(\mathbb{R})$ continuity, we must have

$$\begin{aligned}(\psi^1)'(-a) = (\psi^2)'(-a) &\implies ik\bar{z} - ikBz = \beta C\bar{w} - \beta Dw \\ (\psi^2)'(a) = (\psi^3)'(a) &\implies \beta Cw - \beta D\bar{w} = ikEz\end{aligned}$$

Solving this 4×4 system of equations:

$$\begin{aligned}B &= \frac{\bar{z}(-\bar{w} + w)(\bar{w} + w)(\beta^2 + k^2)}{z(-i\bar{w}\beta + \bar{w}k + i\beta w + kw)(i\bar{w}\beta - \bar{w}k + i\beta w + kw)} \\ C &= -\frac{2\bar{w}\bar{z}k(-i\beta + k)}{(-i\bar{w}\beta + \bar{w}k + i\beta w + kw)(i\bar{w}\beta - \bar{w}k + i\beta w + kw)} \\ D &= \frac{2\bar{z}kw(i\beta + k)}{(-i\bar{w}\beta + \bar{w}k + i\beta w + kw)(i\bar{w}\beta - \bar{w}k + i\beta w + kw)} \\ E &= \frac{4i\bar{z}\beta k}{z(-i\bar{w}\beta + \bar{w}k + i\beta w + kw)(i\bar{w}\beta - \bar{w}k + i\beta w + kw)}\end{aligned}$$

Substituting $w + \bar{w} = 2 \cosh(\beta a)$ and $w - \bar{w} = 2 \sinh(\beta a)$:

$$\begin{aligned}B &= \frac{\bar{z} \cosh(\beta a) \sinh(\beta a)(\beta^2 + k^2)}{z(k \cosh(\beta a) + i\beta \sinh(\beta a))(k \sinh(\beta a) + i\beta \cosh(\beta a))} \\ C &= -\frac{\bar{w}\bar{z}k(-i\beta + k)}{2(k \cosh(\beta a) + i\beta \sinh(\beta a))(k \sinh(\beta a) + i\beta \cosh(\beta a))} \\ D &= \frac{\bar{z}kw(i\beta + k)}{2(k \cosh(\beta a) + i\beta \sinh(\beta a))(k \sinh(\beta a) + i\beta \cosh(\beta a))} \\ E &= \frac{i\bar{z}\beta k}{z(k \cosh(\beta a) + i\beta \sinh(\beta a))(k \sinh(\beta a) + i\beta \cosh(\beta a))}\end{aligned}$$

Expanding the denominator:

$$\begin{aligned}B &= \frac{2\bar{z}^2 \cosh(\beta a) \sinh(\beta a)(\beta^2 + k^2)}{(k^2 - \beta^2) \sinh(2\beta a) + 2\beta k i \cosh(2\beta a)} \\ C &= -\frac{\bar{w}\bar{z}k(-i\beta + k)}{(k^2 - \beta^2) \sinh(2\beta a) + 2\beta k i \cosh(2\beta a)} \\ D &= \frac{\bar{z}kw(i\beta + k)}{(k^2 - \beta^2) \sinh(2\beta a) + 2\beta k i \cosh(2\beta a)} \\ E &= \frac{2i\bar{z}^2\beta k}{(k^2 - \beta^2) \sinh(2\beta a) + 2\beta k i \cosh(2\beta a)}\end{aligned}$$

The maximum amplitude of ψ^1 is $1 + |B|$, and the maximum amplitude of ψ^3 is $|E|$. Thus, the transmission coefficient is

$$\begin{aligned}\tau &= \frac{|E|}{1 + |B|} \\ &= \frac{2\beta k}{2(\beta^2 + k^2) \cosh(\beta a) \sinh(\beta a) + \sqrt{(k^2 - \beta^2)^2 \sinh^2(2\beta a) + 4\beta^2 k^2 \cosh^2(2\beta a)}}.\end{aligned}$$

Problem 3.

(a) We have that

$$\begin{aligned}
\langle x \rangle &= \int_0^L dx \psi_n^* x \psi_n \\
&= \frac{2}{L} \int_0^L dx x \sin\left(\frac{n\pi x}{L}\right)^2 \\
&= \frac{1}{L} \int_0^L dx x \left[1 - \cos\left(\frac{2n\pi x}{L}\right)\right] \\
&= \frac{1}{L} \cdot \frac{L^2}{2} - \int_0^L dx x \cos\left(\frac{2n\pi x}{L}\right) \\
&= \frac{L}{2} - \left[x \frac{L}{2n\pi} \sin\left(\frac{2n\pi x}{L}\right) + \left(\frac{L}{2n\pi}\right)^2 \cos\left(\frac{2n\pi x}{L}\right) \right] \Big|_0^L \quad (\text{repeated IBP}) \\
&= \frac{L}{2}.
\end{aligned}$$

(b) The momentum operator is $\hat{p} = (\hbar/i) \partial/\partial x$, thus

$$\begin{aligned}
\langle p \rangle &= \int_0^L dx \psi_n^* \frac{\hbar}{i} \frac{\partial}{\partial x} \psi_n \\
&= \frac{\hbar}{i} \frac{2}{L} \frac{n\pi}{L} \int_0^L dx \sin\left(\frac{n\pi x}{L}\right) \cos\left(\frac{n\pi x}{L}\right) \\
&= \frac{2n\pi\hbar}{iL^2} \int_0^L dx \sin\left(\frac{2n\pi x}{L}\right) \\
&= 0.
\end{aligned}$$

(c) We have that

$$\begin{aligned}
\langle x^2 \rangle &= \int_0^L dx \psi_n^* x^2 \psi_n \\
&= \frac{2}{L} \int_0^L dx x^2 \sin\left(\frac{n\pi x}{L}\right)^2 \\
&= \frac{1}{L} \int_0^L dx x^2 \left[1 - \cos\left(\frac{2n\pi x}{L}\right)\right] \\
&= \frac{1}{L} \cdot \frac{L^3}{3} - \frac{1}{L} \int_0^L dx x^2 \cos\left(\frac{2n\pi x}{L}\right) \\
&= \frac{L^2}{3} - \frac{1}{L} \left[x^2 \frac{L}{2n\pi} \sin\left(\frac{2n\pi x}{L}\right) + 2x \left(\frac{L}{2n\pi}\right)^2 \cos\left(\frac{2n\pi x}{L}\right) + 2 \left(\frac{L}{2n\pi}\right)^3 \sin\left(\frac{2n\pi x}{L}\right) \right] \Big|_0^L \\
&= \frac{L^2}{3} - 2 \left(\frac{L}{2n\pi}\right)^2 \\
&= \frac{(2n^2\pi^2 - 3)L^2}{6n^2\pi^2}.
\end{aligned}$$

(d) We have that

$$\langle p^2 \rangle = -\hbar^2 \int_0^L dx \psi_n^* \frac{\partial^2}{\partial x^2} \psi_n$$

$$\begin{aligned}
&= \hbar^2 \frac{2}{L} \frac{n^2 \pi^2}{L^2} \int_0^L dx \sin\left(\frac{n\pi x}{L}\right)^2 \\
&= \frac{n^2 \pi^2 \hbar^2}{L^3} \int_0^L dx \left[1 - \cos\left(\frac{n\pi x}{L}\right)\right] \\
&= \frac{n^2 \pi^2 \hbar^2}{L^2}.
\end{aligned}$$

(e) By definition,

$$\begin{aligned}
\Delta x &= \sqrt{\langle x^2 \rangle - \langle x \rangle^2} \\
&= \sqrt{\frac{(2n^2 \pi^2 - 3)L^2}{6n^2 \pi^2} - \frac{L^2}{4}} \\
&= L \sqrt{\frac{4(2n^2 \pi^2 - 3) - 6n^2 \pi^2}{24n^2 \pi^2}} \\
&= \frac{L}{n\pi} \sqrt{\frac{2n^2 \pi^2 - 3}{24}}.
\end{aligned}$$

(f) By definition,

$$\begin{aligned}
\Delta p &= \sqrt{\langle p^2 \rangle - \langle p \rangle^2} \\
&= \sqrt{\frac{n^2 \pi^2 \hbar^2}{L^2}} \\
&= \frac{n\pi \hbar}{L}.
\end{aligned}$$

(g) Thus

$$\begin{aligned}
\Delta x \Delta p &= \hbar \sqrt{\frac{2n^2 \pi^2 - 3}{24}} \\
&= \frac{\hbar}{2} \sqrt{\frac{2n^2 \pi^2 - 3}{6}}.
\end{aligned}$$

The lowest this value can possibly be is when $n = 1$, where

$$\Delta x \Delta p = \frac{\hbar}{2} \sqrt{\frac{2\pi^2 - 3}{6}} \approx 1.67 \cdot \frac{\hbar}{2}.$$

Problem 4.

(a) We have that

$$\begin{aligned}
\langle x \rangle &= \int_{\mathbb{R}} dx \psi_0^* x \psi_0 \\
&= C_0^2 \int_{\mathbb{R}} dx x e^{-2ax^2} \\
&= 0 \quad (\text{odd function}).
\end{aligned}$$

(b) We have that

$$\begin{aligned}
\langle p \rangle &= \frac{\hbar}{i} \int_{\mathbb{R}} dx \psi_0^* \frac{\partial}{\partial x} \psi_0 \\
&= -\frac{2a\hbar}{i} C_0^2 \int_{\mathbb{R}} dx x e^{-2ax^2} \\
&= 0 \quad (\text{odd function}).
\end{aligned}$$

(c) We have that

$$\begin{aligned}
 \langle x^2 \rangle &= \int_{\mathbb{R}} dx \psi_0^* x^2 \psi_0 \\
 &= C_0^2 \int_{\mathbb{R}} dx x^2 e^{-2ax^2} \\
 &= -\frac{C_0^2}{4a} x e^{-2ax^2} \Big|_{-\infty}^{\infty} + \frac{C_0^2}{4a} \int_{\mathbb{R}} dx e^{-2ax^2} \\
 &= \frac{C_0^2}{8} \sqrt{\frac{2\pi}{a}}.
 \end{aligned}$$

(d) We have that

$$\begin{aligned}
 \langle p^2 \rangle &= -\hbar^2 \int_{\mathbb{R}} dx \psi_0^* \frac{\partial^2}{\partial x^2} \psi_0 \\
 &= -\hbar^2 C_0^2 \int_{\mathbb{R}} dx (4a^2 x^2 e^{-2ax^2} - 2ae^{-2ax^2}) \\
 &= \sqrt{2\pi a} \hbar^2 C_0^2 - \frac{\sqrt{2\pi a}}{2} \hbar^2 C_0^2 \\
 &= \frac{\sqrt{2\pi a}}{2} C_0^2 \hbar^2 \\
 &= \sqrt{\frac{\pi a}{2}} C_0^2 \hbar^2
 \end{aligned}$$

(e) We have that

$$\begin{aligned}
 \Delta x &= \sqrt{\langle x^2 \rangle - \langle x \rangle^2} \\
 &= \sqrt{\frac{C_0^2}{8} \sqrt{\frac{2\pi}{a}} - 0^2} \\
 &= \frac{2^{3/4} \pi^{1/4} C_0}{4a^{1/4}}
 \end{aligned}$$

(f) We have that

$$\begin{aligned}
 \Delta p &= \sqrt{\langle p^2 \rangle - \langle p \rangle^2} \\
 &= \sqrt{\sqrt{\frac{\pi a}{2}} C_0^2 \hbar^2 - 0^2} \\
 &= \left(\frac{\pi a}{2}\right)^{1/4} C_0 \hbar.
 \end{aligned}$$

(g) Therefore,

$$\begin{aligned}
 \Delta x \Delta p &= \frac{2^{3/4} \pi^{1/4} C_0}{4a^{1/4}} \left(\frac{\pi a}{2}\right)^{1/4} C_0 \hbar \\
 &= \frac{\pi^{1/2} C_0^2 \hbar}{2a^{1/2} 2} \\
 &= \frac{\sqrt{2}}{4} \hbar \quad (???)
 \end{aligned}$$